src/Logic/APL.v
@@ -1,0 +1,179 @@
+
+Require Import Coq.Classes.RelationClasses.
+Require Import Coq.Classes.Morphisms.
+Require Import stdpp.base.
+
+Reserved Notation "'emp'".
+Reserved Notation "(⊢)" (at level 99).
+Reserved Notation "P ⊢ Q" (at level 99, Q at level 200, right associativity).
+Reserved Notation "P ∧ Q" (at level 80, right associativity, format "P '/' ∧ '/' Q").
+Reserved Notation "P ∨ Q" (at level 85, right associativity, format "P '/' ∨ '/' Q").
+Reserved Notation "P → Q"
+(at level 99, Q at level 200, right associativity,
+ format "'[' P '/' → '/' '[' Q ']' ']'").
+
+
+
+Local Set Primitive Projections.
+Module APL.
+    Universe Logic.
+    Universe Quant.
+
+    Section laws.
+        Context {PROP : Type}.
+    
+        Context {apl_entails : PROP -> PROP -> Prop}.
+        Context {apl_and : PROP -> PROP -> PROP}.
+        Context {apl_imp: PROP -> PROP -> PROP}.
+        Context {apl_forall : forall A, (A -> PROP) -> PROP}.
+
+        Bind Scope apl_scope with PROP.
+
+
+        Local Infix "⊢" := apl_entails.
+        Local Infix "∧" := apl_and : apl_scope.
+        Local Infix "→" := apl_imp : apl_scope.
+
+        Record AplLaws := {
+            apl_entails_po : PreOrder apl_entails ;
+
+            apl_and_elim_l P Q : P ∧ Q ⊢ P;
+            apl_and_elim_r P Q : P ∧ Q ⊢ Q;
+            apl_and_intro P Q R : (P ⊢ Q) -> (P ⊢ R) -> P ⊢ Q ∧ R;
+
+            apl_impl_intro_r P Q R : (P ∧ Q ⊢ R) -> P ⊢ Q → R;
+            apl_impl_elim_l' P Q R : (P ⊢ Q → R) -> P ∧ Q ⊢ R;
+
+            apl_forall_term_intro {A} P (Ψ : A -> PROP) : 
+                (forall a, P ⊢ Ψ a) -> P ⊢ apl_forall _ (fun a => Ψ a );
+        }.
+    End laws.
+
+    Structure apl := APL {
+        apl_car :> Type@{Logic};
+        apl_entails : apl_car -> apl_car -> Prop;
+        apl_emp : apl_car;
+        (* equality *)
+        (* relations *)
+        apl_imp : apl_car -> apl_car -> apl_car ;
+        apl_forall :  forall A : Type@{Quant}, (A -> apl_car) -> apl_car;
+(*         (* forall term *)
+        apl_forall_term : forall A : Type@{Quant}, (A -> apl_car) -> apl_car;
+        (* forall type *)
+        apl_forall_type : forall A : Type@{Quant}, (A -> apl_car) -> apl_car;
+        (* forall rel *)
+        apl_forall_rel : forall A : Type@{Quant}, (A -> apl_car) -> apl_car; *)
+        apl_and : apl_car -> apl_car -> apl_car;
+        apl_or : apl_car -> apl_car -> apl_car;
+        apl_exist : forall A : Type@{Quant}, (A -> apl_car) -> apl_car;
+        (* exists term *)
+(*         apl_exist_term : forall A : Type@{Quant}, (A -> apl_car) -> apl_car;
+        (* exists type *)
+        apl_exist_type : forall A : Type@{Quant}, (A -> apl_car) -> apl_car;
+        (* exists rel *)
+        apl_exist_rel : forall A : Type@{Quant}, (A -> apl_car) -> apl_car; *)
+        apl_laws : @AplLaws apl_car apl_entails apl_and apl_imp apl_forall
+    }.
+
+    Declare Scope apl_scope.
+    (* https://plv.mpi-sws.org/coqdoc/iris/iris.bi.interface.html#bi_cofe *)
+    Delimit Scope apl_scope with A.
+    Bind Scope apl_scope with apl_car.
+
+    Global Instance: Params (@apl_entails) 1 := {}.
+    Global Instance: Params (@apl_emp) 1 := {}.
+    Global Instance: Params (@apl_and) 1 := {}.
+    Global Instance: Params (@apl_imp) 1 := {}.
+    Global Instance: Params (@apl_forall) 2 := {}.
+    Global Instance: Params (@apl_exist) 2 := {}.
+
+    Global Arguments apl_car : simpl never.
+    Global Arguments apl_entails {PROP} _ _ : simpl never, rename.
+    Global Arguments apl_emp {PROP} : simpl never, rename.
+    Global Arguments apl_and {PROP} _ _ : simpl never, rename.
+    Global Arguments apl_or {PROP} _ _ : simpl never, rename.
+    Global Arguments apl_imp {PROP} _ _ : simpl never, rename.
+    Global Arguments apl_forall {PROP _} _%_A : simpl never, rename.
+    Global Arguments apl_exist {PROP _} _%_A : simpl never, rename.
+
+    Notation "'emp'" := (apl_emp) : apl_scope.
+    Infix "∧" := apl_and : apl_scope.
+    Notation "(∧)" := apl_and (only parsing) : apl_scope.
+    Infix "∨" := apl_or : apl_scope.
+    Notation "(∨)" := apl_or (only parsing) : apl_scope.
+    Infix "→" := apl_imp : apl_scope.
+(* 
+    Notation "∀ x .. y , P" :=
+    (apl_forall (λ x, .. (apl_forall (λ y, P%I)) ..)) : apl_scope.
+    Notation "∃ x .. y , P" :=
+    (apl_exist (λ x, .. (apl_exist (λ y, P%I)) ..)) : apl_scope. *)
+    Notation "(⊢)" := apl_entails (only parsing) : stdpp_scope.
+    Notation "P ⊢ Q" := (apl_entails P%A Q%A) : stdpp_scope.
+
+    Definition apl_emp_valid {PROP : apl} (P : PROP) : Prop := emp ⊢ P.
+
+    Global Arguments apl_emp_valid {_} _%_A : simpl never.
+    Global Typeclasses Opaque apl_emp_valid.
+    
+    Notation "⊢ Q" := (apl_emp_valid Q%A) (at level 99) : stdpp_scope.
+(*     Notation "'⊢@{' PROP } Q" := (apl_emp_valid (PROP:=PROP) Q%I) (only parsing) (at level 99): stdpp_scope.
+ *)
+
+    (* https://plv.mpi-sws.org/coqdoc/iris/iris.bi.interface.html#::bi_scope:'emp' *)
+
+    
+
+    Check apl_and.
+    Fail Definition thing P Q  := (True ∧ Q)%A.
+    Fail Definition thing P Q  := (⊢ P ∧ Q)%A.
+ 
+End APL.
+
+Import APL.
+Check @AplLaws.
+
+Check or.
+Locate and.
+
+(* Woah...  *)
+Print Logic.
+
+
+Definition imp (A B : Prop) := forall (_ : A ), B.
+
+Check @AplLaws Prop imp and imp all.
+
+Lemma instance : @AplLaws Prop imp and imp all.
+Proof.
+    constructor; unfold imp in *.
+    (* These laws already exist in Logic module *)
+    2:{ intros P Q [P' Q']. exact P'.  }
+    6:{ intros. unfold all. intros. pose proof (H x H0). exact H1. }
+Admitted.
+
+Section huh.
+    Context {PROP : apl}.
+    Context {term : Type}.
+    Check @apl_imp PROP.
+    Check apl_imp.
+    Notation "P ⊢ Q" := (@apl_entails PROP P%A Q%A) : stdpp_scope.
+    Infix "∧" := (@apl_and PROP ): apl_scope.
+
+    Check imp.
+
+
+Fail Lemma  thing (P Q : PROP) : ⊢ ((Q → True) ∧ Q)%A.
+
+Lemma thing P Q  : P ∧ (P → Q)⊢ Q.
+Proof.
+    Check apl_and_intro (apl_laws PROP).
+    Check apl_impl_elim_l' (apl_laws PROP).
+    apply (apl_impl_elim_l' (apl_laws PROP)).
+Abort.
+
+Lemma foo P : ⊢ @apl_forall PROP term (fun x => P).
+Proof.
+    apply (apl_forall_term_intro (apl_laws PROP)).
+    intros.
+    Check apl_forall_term_intro (apl_laws PROP).
+Check @apl_forall PROP term.
