src/OSum/PolyG.v
@@ -1,0 +1,43 @@
+Require Import Autosubst.Autosubst.
+
+
+Module PolyG.
+(* PolyC would add TTag : type *)
+Inductive type :=
+    | TDyn : type
+    | TVar (x : var)
+    | TUnit
+    | TBool : type
+    | TProd (x y : type)
+    | TArrow (x y : type)
+    | TExistNew (x : {bind type})
+    | TForallNew (x : {bind type}).
+
+Inductive groundTy := 
+    | GVar 
+    | GBool 
+    | GProd 
+    | GArr 
+    | GExist 
+    | GForall.
+
+Inductive expr := 
+    | Var (x : var)
+    | Ascript (e : expr)(t : type)
+    | Seal (t : type)(e : expr)
+    | Unseal (t : type)(e : expr)
+    | TagTest (g : groundTy) (e : expr)
+    | Let (e1 : expr) (e2 : {bind expr})
+    | Bool (b : bool)
+    | If (e1 e2 e3 : expr)
+    | Pair (e1 e2 : expr)
+    | PairElim (e1 : expr)(e2 : {bind (expr * expr)})
+    | Lam (e : {bind expr})
+    | App (e1 e2 : expr)
+    | Pack (e : expr)
+    | Unpack (e1 : expr)(e2 : {bind expr})
+    | TLam (e : expr)
+    | TApp (e1 : expr)(e2 : {bind expr}).
+
+
+End PolyG.
