src/OSum/PolyG_binrel.v
@@ -1,0 +1,308 @@
+From stdpp Require Import base gmap coPset tactics proof_irrel.
+
+From iris.base_logic Require Import invariants iprop upred saved_prop gen_heap.
+From iris.base_logic.lib Require Import ghost_map gset_bij.
+From iris.algebra Require Import cofe_solver gset gmap_view excl gset_bij.
+From iris.proofmode Require Import proofmode.
+From iris.program_logic Require Import weakestpre.
+Require Import Autosubst.Autosubst.
+
+From MyProject.src.OSum Require Export PolyG OSum persistent_pred wp_rules binary_rules.
+
+Module PolyGBinRel.
+
+    Definition combine {A}{B}`{Countable (A * B)}(l : list A)(l' : list B) : gset (A * B) := 
+        list_to_set (zip l l').
+
+
+    Lemma not_in_combine_left {A}{B}`{Countable (A * B)}(l1 : list A)(l2 : list B) a b : 
+        a ∉ l1 -> 
+        (a , b) ∉ combine l1 l2 .
+    Proof.
+        unfold not. intros.
+        apply elem_of_list_to_set in H1.
+        apply elem_of_zip_l in H1.
+        apply H0. exact H1. 
+    Qed.
+
+    Lemma not_in_combine_right {A}{B}`{Countable (A * B)}(l1 : list A)(l2 : list B) a b : 
+        b ∉ l2 -> 
+        (a , b) ∉ combine l1 l2 .
+    Proof.
+        unfold not. intros.
+        apply elem_of_list_to_set in H1.
+        apply elem_of_zip_r in H1.
+        apply H0. exact H1. 
+    Qed.
+
+    Lemma adjust_combine {A B}`{Countable (A * B)}{L1 L2} a b :
+        a ∉ L1 -> 
+        b ∉ L2 -> 
+        {[(a, b)]} ∪ combine L1 L2 = combine (a :: L1) (b :: L2).
+    Proof.
+        intros.
+        rewrite set_eq.
+        intros (a' , b').
+        split.
+        - intros. 
+        destruct (decide ((a , b) = (a' , b'))).
+        {
+            inversion e. subst.
+            apply elem_of_list_to_set.
+            rewrite (zip_with_app pair [a'] L1 [b'] L2 eq_refl).
+            constructor.
+        }
+        apply elem_of_list_to_set.
+        pose proof (zip_with_app pair [a] L1 [b] L2 eq_refl).
+        rewrite H3.
+        apply elem_of_list_further.
+        pose proof ( elem_of_union {[(a, b)]} (combine L1 L2) (a' , b')).
+        apply H4 in H2.
+        destruct H2.
+        +        assert ( (a , b) <> (a' , b')). {
+            unfold not. intros. inversion H5. apply n. done.
+        }
+        rewrite elem_of_singleton in H2. symmetry in H2. contradiction.
+        + unfold combine in H2.            
+        apply elem_of_list_to_set in H2. exact H2.
+        -
+        intros.
+        unfold combine in H2. apply elem_of_list_to_set in H2.
+        simpl in H2.
+        unfold combine.
+        Search list_to_set.
+        rewrite <- list_to_set_cons.
+        apply elem_of_list_to_set. exact H2.
+    Qed.
+
+    Definition logN : namespace := nroot .@ "logN".
+
+    Class RelationResources Σ := RelRes{
+        predicates :: savedPredG Σ (val * val) ;
+        rel_bijection :: gset_bijG Σ (loc * loc) loc ;
+        name_bijection :: gset_bijG Σ loc loc;
+        sets :: inG Σ (authR (gsetUR loc))
+    }.
+
+    Class relStore  Σ  := RelStore {
+        resources :: RelationResources Σ ; 
+        rel_bij : gname ;
+        name_bij : gname; 
+        name_set : gname
+    }.
+
+    Class logrelSig Σ := LogRelSig {
+        invariants : invGS Σ;
+        store :: relStore  Σ ;
+    }.
+
+    Notation Gtype := MyProject.src.OSum.PolyG.PolyG.type.
+
+    Definition D `{ts : !relStore Σ}:= persistent_pred (val * val) (iProp Σ).
+
+    Definition state_interp  `{relStore Σ}`{configSpec Σ}(s : list loc) : iProp Σ :=
+        ∃ (s' s'': list loc ) , 
+            own config_name (◯ (None, list_to_set s')) ∗
+            gset_bij_own_auth name_bij (DfracOwn 1) (combine s s') ∗
+            gset_bij_own_auth rel_bij (DfracOwn 1) (combine (zip s s') s'') ∗
+            [∗ list] l ∈ s'', (∃ (P : D), saved_pred_own l (DfracDiscarded) P).
+
+    Global Instance OSum_irisGS `{logrelSig Σ}`{configSpec Σ} : irisGS OSum_lang Σ := {
+            iris_invGS := invariants;
+            num_laters_per_step _ := 0;
+            state_interp s  _ _ _ := state_interp s;
+            fork_post _ := True%I;
+            state_interp_mono _ _ _ _ := fupd_intro _ _
+    }.
+
+Section binary_rel.
+    Context `{logrelSig Σ, configSpec Σ}.
+
+    Definition VRel := listO D -n> D.
+
+    Program Definition pointsto_def (l l' : loc) : D -n> iPropO Σ  :=
+    λne R, (∃ (l'' : loc), 
+            gset_bij_own_elem name_bij l l'  ∗
+            gset_bij_own_elem rel_bij (l , l') l''  ∗ 
+            saved_pred_own l'' DfracDiscarded R)%I.
+    Next Obligation. Admitted.
+
+    Notation "l @ l' ↦□ R" := (pointsto_def l l' R)
+    (at level 20,  format "l @ l' ↦□ R") : bi_scope.
+
+    Instance mypointsto_persist (l l': loc)  (R : D) : Persistent (l @ l' ↦□ R).
+    apply _. Qed.
+
+    Definition interp_expr (τi :  VRel) (Δ : listO D) (ee : expr * expr) : iProp Σ := 
+    (∀ K, ⤇ fill K (ee.2) -∗
+        WP ee.1 {{ v, ∃ v', ⤇ fill K (of_val v') ∧ τi Δ (v, v') }})%I.
+
+    Global Instance interp_expr_ne n :
+        Proper (dist n ==> dist n ==> (=) ==> dist n) interp_expr.
+    Proof. unfold interp_expr; solve_proper. Qed.
+
+    Definition interp_TDyn : VRel := 
+        λne rho, PersPred(fun w => 
+            ∃ (l l' : loc)(v1 v2 : val)(R : D),
+                ⌜w = (InjV (CaseV l) v1 , InjV (CaseV l') v2)⌝ ∧
+                ▷ l @ l' ↦□ R ∧
+                R (v1 ,v2))%I.
+
+    Program Definition interp_TVar (v : var) : VRel := 
+        λne rho, PersPred (default (inhabitant : persistent_pred _ _) (rho !! v)).
+    Solve Obligations with repeat intros ?; simpl; solve_proper.
+
+    Definition interp_TBool : VRel := 
+    λne rho, PersPred(fun w => (∃ (b : bool), ⌜w.1 = BoolV b /\ w.2 = BoolV b⌝))%I.
+
+    Program Definition interp_TProd (interp1 interp2 : VRel) : VRel := 
+        λne rho, PersPred(fun w => (∃ vv1 vv2 , 
+            ⌜w = (PairV vv1.1 vv2.1 ,PairV vv1.2 vv2.2)⌝  ∧ 
+            interp1 rho vv1  ∧ 
+            interp2 rho vv2))%I.  
+    Solve Obligations with solve_proper.
+    
+    Program Definition interp_TArrow (interp1 interp2 : VRel) : VRel :=
+        λne Δ,
+        PersPred
+        (λ ww, □ ∀ vv, |==> interp1 Δ vv →
+                        interp_expr
+                            interp2 Δ (App (of_val (ww.1)) (of_val (vv.1)),
+                                        App (of_val (ww.2)) (of_val (vv.2))))%I.
+    Solve Obligations with solve_proper.
+
+    (* equality of functions...? *)
+    Program Definition interp_TExistNew (interp : VRel) : VRel :=
+        λne Δ,PersPred
+            (λ ww, ∃ vv (R : D) , ⌜ww = (PackV vv.1, PackV vv.2)⌝ ∗ 
+            □  ∀ (sig1 sig2 : loc), 
+            |==> sig1 @ sig2 ↦□ R →
+                    interp_expr interp (R :: Δ) 
+                    ((App (of_val vv.1) (Case sig1)), (App (of_val vv.2) (Case sig2))))%I.
+    Solve Obligations with repeat intros ?; simpl; solve_proper.
+
+    Program Definition interp_TForallNew (interp : VRel) : VRel := 
+        λne Δ, PersPred(fun ww =>
+        □ ∀ (R : D) (sig1 sig2 : loc),
+            |==> sig1 @ sig2 ↦□ R →
+            interp_expr
+            interp (R :: Δ) (App (TApp (of_val (ww.1))) (Case sig1), (App (TApp (of_val (ww.2))) (Case sig2))))%I.
+    Solve Obligations with solve_proper.
+
+    Fixpoint interp (τ : Gtype) : VRel :=
+        match τ return _ with
+            | PolyG.TDyn => interp_TDyn
+            | PolyG.TVar x => interp_TVar x
+            | PolyG.TBool => interp_TBool
+            | PolyG.TProd t1 t2 => interp_TProd (interp t1) (interp t2)
+            | PolyG.TArrow t1 t2 => interp_TArrow (interp t1) (interp t2)
+            | PolyG.TExistNew t => interp_TForallNew (interp t)
+            | PolyG.TForallNew t => interp_TExistNew (interp t)
+        end.
+
+        Notation "⟦ τ ⟧" := (interp τ).
+
+        Notation "⟦ τ ⟧ₑ" := (interp_expr (interp τ)).
+    
+    End binary_rel.
+    
+ 
+ 
+ End PolyGBinRel.
+   (*  
+        Definition interp_env (Γ : list type)
+        (Δ : list D) (vs : list (val * val)) : iProp Σ :=
+        (⌜length Γ = length vs⌝ ∗ [∗] zip_with (λ τ, ⟦ τ ⟧ Δ) Γ vs)%I.
+        Notation "⟦ Γ ⟧*" := (interp_env Γ).
+    
+        Global Instance interp_env_base_persistent Δ Γ vs :
+        TCForall Persistent (zip_with (λ τ, ⟦ τ ⟧ Δ) Γ vs).
+        Proof. revert vs; induction Γ => vs; destruct vs; constructor; apply _. Qed.
+        Global Instance interp_env_persistent Γ Δ vs : Persistent (⟦ Γ ⟧* Δ vs) := _.
+    
+    
+        Lemma interp_env_nil Δ : ⊢ ⟦ [] ⟧* Δ [].
+        Proof. iSplit; simpl; auto. Qed.
+    
+        Import uPred.
+        Lemma interp_env_cons Δ Γ vvs τ vv :
+            ⟦ τ :: Γ ⟧* Δ (vv :: vvs) ⊣⊢ ⟦ τ ⟧ Δ vv ∗ ⟦ Γ ⟧* Δ vvs.
+        Proof.
+            rewrite /interp_env /= (assoc _ (⟦ _ ⟧ _ _)) -(comm _ ⌜(_ = _)⌝%I) -assoc.
+            by apply sep_proper; [apply pure_proper; lia|].
+        Qed.
+    
+    
+        Lemma interp_env_length Δ Γ vs : ⟦ Γ ⟧* Δ vs ⊢ ⌜length Γ = length vs⌝.
+        Proof. by iIntros "[% ?]". Qed.
+    
+        Lemma interp_env_Some_l Δ Γ vs x τ :
+            Γ !! x = Some τ → ⟦ Γ ⟧* Δ vs ⊢ ∃ v, ⌜vs !! x = Some v⌝ ∧ ⟦ τ ⟧ Δ v.
+        Proof.
+            iIntros (?) "[Hlen HΓ]"; iDestruct "Hlen" as %Hlen.
+            destruct (lookup_lt_is_Some_2 vs x) as [v Hv].
+            { by rewrite -Hlen; apply lookup_lt_Some with τ. }
+            iExists v; iSplit; first done. iApply (big_sepL_elem_of with "HΓ").
+            apply elem_of_list_lookup_2 with x.
+            rewrite lookup_zip_with; by simplify_option_eq.
+        Qed.
+    
+        (*  need to fix this proof *)
+        Lemma interp_weaken Δ1 Π Δ2 τ :
+            ⟦ τ.[upn (length Δ1) (ren (+ length Π))] ⟧ (Δ1 ++ Π ++ Δ2)
+            ≡ ⟦ τ ⟧ (Δ1 ++ Δ2).
+        Proof.
+            revert Δ1 Π Δ2. induction τ=> Δ1 Π Δ2; simpl; auto; intros ?; simpl.
+            - by repeat (f_equiv; try match goal with IH : ∀ _, _ |- _ => by apply IH end).
+            - 
+            Admitted.
+        (*     - by repeat (f_equiv; try match goal with IH : ∀ _, _ |- _ => by apply IH end).
+            - f_equiv.
+            apply fixpoint_proper=> τi w /=.
+            by repeat (f_equiv; try match goal with IH : ∀ _, _ |- _ => by apply (IH (_ :: _)) end).
+            - rewrite iter_up; destruct lt_dec as [Hl | Hl]; simpl.
+            { by rewrite !lookup_app_l. }
+            rewrite !lookup_app_r; [|lia ..]; do 3 f_equiv; lia.
+            - by repeat (f_equiv; try match goal with IH : ∀ _, _ |- _ => by apply (IH (_ :: _)) end).
+            - by repeat (f_equiv; try match goal with IH : ∀ _, _ |- _ => by apply (IH (_ :: _)) end).
+            - by repeat (f_equiv; try match goal with IH : ∀ _, _ |- _ => by apply IH end).
+        Qed. *)
+    
+        (* need to fix this proof  *)
+        Lemma interp_subst_up Δ1 Δ2 τ τ' :
+            ⟦ τ ⟧ (Δ1 ++ interp τ' Δ2 :: Δ2)
+            ≡ ⟦ τ.[upn (length Δ1) (τ' .: ids)] ⟧ (Δ1 ++ Δ2).
+        Proof.
+            revert Δ1 Δ2; induction τ=> Δ1 Δ2; simpl; auto; intros ?; simpl.
+            - by repeat (f_equiv; try match goal with IH : ∀ _, _ |- _ => by apply IH end).
+            - 
+            Admitted. (* by repeat (f_equiv; try match goal with IH : ∀ _, _ |- _ => by apply IH end).
+            - f_equiv.
+            apply fixpoint_proper=> τi w /=.
+            by repeat (f_equiv; try match goal with IH : ∀ _, _ |- _ => by apply (IH (_ :: _)) end).
+            - match goal with |- context [_ !! ?x] => rename x into idx end.
+            rewrite iter_up; destruct lt_dec as [Hl | Hl]; simpl.
+            { by rewrite !lookup_app_l. }
+            rewrite !lookup_app_r; [|lia ..].
+            case EQ: (idx - length Δ1) => [|n]; simpl.
+            { symmetry. asimpl. apply (interp_weaken [] Δ1 Δ2 τ'). }
+            rewrite !lookup_app_r; [|lia ..]. do 3 f_equiv. lia.
+            - by repeat (f_equiv; try match goal with IH : ∀ _, _ |- _ => by apply (IH (_ :: _)) end).
+            - by repeat (f_equiv; try match goal with IH : ∀ _, _ |- _ => by apply (IH (_ :: _)) end).
+            - by repeat (f_equiv; try match goal with IH : ∀ _, _ |- _ => by apply IH end).
+        Qed. *)
+    
+        (* fix this  *)
+        Lemma interp_subst Δ2 τ τ' v : ⟦ τ ⟧ (⟦ τ' ⟧ Δ2 :: Δ2) v ≡ ⟦ τ.[τ'/] ⟧ Δ2 v.
+        Admitted.
+     *)
+    
+(*     End binary_logrel.
+    
+   (*  Global Typeclasses Opaque interp_env.
+    Notation "⟦ τ ⟧" := (interp τ).
+    Notation "⟦ τ ⟧ₑ" := (interp_expr (interp τ)).
+    Notation "⟦ Γ ⟧*" := (interp_env Γ). *)
+
+
+End PolyGBinRel. *)
